LeanSubst/Basic.lean
@@ -1,0 +1,44 @@
+
+namespace LeanSubst
+
+universe u1 u2
+variable {S : Type u1} {T : Type u2}
+
+structure Ren (T : Type u2) where
+  act : Nat -> Nat
+
+class RenMap (S : Type u1) (T : Type u2) where
+  rmap : Ren T -> S -> S
+
+export RenMap (rmap)
+
+macro:max t:term noWs "⟨" r:term "⟩" : term => `(rmap $r $t)
+
+@[app_unexpander rmap]
+def unexpand_rmap : Lean.PrettyPrinter.Unexpander
+| `($_ $r $t) => `($t⟨$r⟩)
+| _ => throw ()
+
+inductive Action (T : Type u2) where
+| re : Nat -> Action T
+| su : T -> Action T
+deriving Repr
+
+export Action (re su)
+
+structure Subst (T : Type u2) where
+  act : Nat -> Action T
+
+class SubstMap (S : Type u1) (T : Type u2) where
+  smap : Subst T -> S -> S
+
+export SubstMap (smap)
+
+macro:max t:term noWs "[" σ:term "]" : term => `(smap $σ $t)
+
+@[app_unexpander smap]
+def unexpand_smap : Lean.PrettyPrinter.Unexpander
+| `($_ $σ $t) => `($t[$σ])
+| _ => throw ()
+
+end LeanSubst
