LeanSubst/Laws.lean
@@ -1,0 +1,409 @@
+
+import LeanSubst.Basic
+import LeanSubst.Ops
+
+namespace LeanSubst
+
+universe u1 u2 u3
+variable {S : Type u1} {T : Type u2} {U : Type u3}
+
+class RenMapId (S : Type u1) (T : Type u2) [RenMap S T] where
+  apply_id {s : S} : s⟨.id T⟩ = s
+
+class RenMapCompose (S : Type u1) (T : Type u2) [RenMap S T] where
+  apply_compose {s : S} {r1 r2 : Ren T} : s⟨r1⟩⟨r2⟩ = s⟨r1 ∘ r2⟩
+
+@[simp]
+theorem Ren.apply_id [RenMap S T] [RenMapId S T] {s : S} : s⟨id T⟩ = s := RenMapId.apply_id
+
+@[simp, grind =]
+theorem Ren.apply_compose [RenMap S T] [RenMapCompose S T] {s : S} {r1 r2 : Ren T}
+  : s⟨r1⟩⟨r2⟩ = s⟨r1 ∘ r2⟩
+:= RenMapCompose.apply_compose
+
+instance (priority := high) [RenMap T T] [RenMapId T T] : RenMapId (Action T) T where
+  apply_id := by intro s; cases s <;> simp
+
+instance [RenMap S T] [RenMapId S T] : RenMapId (Action S) T where
+  apply_id := by intro s; cases s <;> simp
+
+instance (priority := high) [RenMap T T] [RenMapCompose T T] : RenMapCompose (Action T) T where
+  apply_compose := by intro s; cases s <;> simp
+
+instance [RenMap S T] [RenMapCompose S T] : RenMapCompose (Action S) T where
+  apply_compose := by intro s; cases s <;> simp
+
+class SubstMapId (S : Type u1) (T : Type u2) [SubstMap S T] where
+  apply_id {s : S} : s[.id T] = s
+
+class SubstMapStable (S : Type u1) (T : Type u2) [RenMap S T] [SubstMap S T] where
+  apply_stable (r : Ren T) (σ : Subst T) : r.to = σ -> rmap (S := S) r = smap σ
+
+class SubstMapRenComposeLeft (S : Type u1) (T : Type u2) [RenMap S T] [SubstMap S T] where
+  apply_ren_compose_left {s : S} {r : Ren T} {τ : Subst T} : s⟨r⟩[τ] = s[r ∘ τ]
+
+class SubstMapRenComposeRight (T : Type u2) [RenMap T T] [SubstMap T T] where
+  apply_ren_compose_right {t : T} {r : Ren T} {σ : Subst T} : t[σ]⟨r⟩ = t[σ ∘ r]
+
+class SubstMapCompose (S : Type u1) (T : Type u2) [SubstMap S T] [SubstMap T T] where
+  apply_compose {s : S} {σ τ : Subst T} : s[σ][τ] = s[σ ∘ τ]
+
+class SubstMapRenCommute (S : Type u1) (T : Type u2) [RenMap S S] [SubstMap S T] where
+  apply_ren_commute {s : S} (r : Ren S) (τ : Subst T) : s⟨r⟩[τ] = s[τ]⟨r⟩
+
+class SubstMapHetCompose (S : Type u1) (T : Type u2) [SubstMap S S] [SubstMap S T] where
+  apply_hcompose {s : S} {σ : Subst S} {τ : Subst T} : s[σ][τ] = s[τ][σ ◾ τ]
+
+namespace Subst
+  export SubstMapStable (apply_stable)
+  export SubstMapRenComposeLeft (apply_ren_compose_left)
+  export SubstMapRenComposeRight (apply_ren_compose_right)
+  export SubstMapRenCommute (apply_ren_commute)
+end Subst
+
+@[grind <-]
+theorem Ren.lift_eq_from_eq [RenMap T T] {r : Ren T} {σ : Subst T}
+  : r.to = σ -> r.to.lift = σ.lift
+:= by intro h; rw [<-h]
+
+namespace Subst
+  section
+    @[simp, grind =]
+    theorem rewrite1 : re 0 :: +1 = id T := by
+      simp [Subst.cons, Subst.id]
+      funext; case _ x =>
+      cases x; all_goals simp
+
+    open SubstMap
+
+    @[simp, grind =]
+    theorem I_lift [RenMap T T] {k} : +0.lift k = id T := by
+      funext; case _ x =>
+      cases x; all_goals (simp [Subst.lift, Subst.id])
+      grind
+
+    @[simp, grind =]
+    theorem rewrite2 [SubstMap T T] {σ : Subst T} : +0 ∘ σ = σ := by
+      funext; case _ x =>
+      unfold Subst.compose; simp [Subst.id]
+
+    @[simp, grind =]
+    theorem rewrite3_replace [SubstMap T T] {σ τ : Subst T} {s : T}
+      : (su s :: σ) ∘ τ = su s[τ] :: (σ ∘ τ)
+    := by
+      simp [Subst.cons, Subst.compose]
+      funext; case _ x =>
+      cases x; all_goals simp
+
+    @[simp, grind =]
+    theorem rewrite3_rename [SubstMap T T] {s} {σ τ : Subst T}
+      : (re s :: σ) ∘ τ = (τ.act s) :: (σ ∘ τ)
+    := by
+      simp [Subst.cons, Subst.compose]
+      funext; case _ x =>
+      cases x; all_goals simp
+
+    @[simp, grind =]
+    theorem rewrite4 [SubstMap T T]  {s} {σ : Subst T} : +1 ∘ (s :: σ) = σ := by
+      simp [Subst.cons]
+      funext; case _ x =>
+      cases x; all_goals (simp [Subst.compose, Subst.succ])
+
+    @[simp, grind =]
+    theorem rewrite5 [SubstMap T T] {σ : Subst T} : σ.act 0 :: (+1 ∘ σ) = σ := by
+      simp [Subst.cons, Subst.compose]; congr
+      funext; case _ x =>
+      cases x <;> simp
+  end
+
+  @[simp, grind =]
+  theorem apply_I_is_id [SubstMap S T] [SubstMapId S T] {s : S}
+    : s[id T] = s
+  := SubstMapId.apply_id
+
+  @[simp, grind =]
+  theorem rewrite_lift [RenMap T T] [SubstMap T T] [SubstMapStable T T] {σ : Subst T}
+    : σ.lift = re 0 :: (σ ∘ +1)
+  := by
+    simp [Subst.cons, Subst.lift, Subst.compose]
+    funext; case _ x =>
+    cases x; simp
+    case _ n =>
+      simp [Subst.succ]
+      generalize tdef : σ.act n = t
+      cases t <;> simp at *
+      case _ y =>
+        rw [apply_stable (σ := +1)]
+        simp [Subst.succ]
+        rw [Ren.to_succ]
+
+  @[simp, grind =]
+  theorem rewrite_lift_zero [RenMap T T] [RenMapId T T] {σ : Subst T}
+    : σ.lift 0 = σ
+  := by simp [Subst.lift]
+
+  @[grind =]
+  theorem rewrite_lift_succ
+    [RenMap T T] [RenMapId T T] [RenMapCompose T T]
+    {k} {σ : Subst T}
+    : σ.lift (k + 1) = (σ.lift k).lift
+  := by
+    induction k; simp
+    case _ n ih =>
+      replace ih i : (σ.lift (n + 1)).act i = ((σ.lift n).lift 1).act i := by rw [ih]
+      simp [Subst.lift]
+      funext; case _ i =>
+      have lem := ih i
+      cases i <;> simp
+      case _ i =>
+        simp [Subst.lift] at lem
+        split; simp; case _ h1 =>
+        simp at h1
+        have lem2 : n ≤ i := by omega
+        generalize zdef : σ.act (i - (n + 1)) = z
+        cases z <;> simp; omega
+        congr
+
+  @[simp, grind =]
+  theorem rewrite6 [RenMap T T] [SubstMap T T] [SubstMapId T T] {σ : Subst T}
+    : σ ∘ +0 = σ
+  := by
+    simp [Subst.compose, Subst.id]; congr
+    funext; case _ x =>
+    generalize zdef : σ.act x = z
+    cases z <;> simp at *; case _ s =>
+    have lem := SubstMapId.apply_id (T := T) (s := s)
+    simp [Subst.id] at lem; exact lem
+
+  @[simp, grind =]
+  theorem apply_compose [SubstMap S T] [SubstMap T T] [SubstMapCompose S T] {s : S} {σ τ : Subst T}
+    : s[σ][τ] = s[σ ∘ τ]
+  := SubstMapCompose.apply_compose
+
+  @[simp, grind =]
+  theorem rewrite7
+    [SubstMap T T] [SubstMapCompose T T]
+    {σ τ μ : Subst T}
+    : (σ ∘ τ) ∘ μ = σ ∘ τ ∘ μ
+  := by
+    simp [Subst.compose]
+    funext; case _ x =>
+    cases σ.act x <;> simp [Subst.compose]
+
+  @[simp, grind =]
+  theorem hrewrite1 [SubstMap S T] [SubstMapId S T] {σ : Subst S} : σ ◾ (id T) = σ := by
+    simp [Subst.hcompose]; congr
+    funext; case _ x =>
+    generalize zdef : σ.act x = z
+    cases z <;> simp
+
+  -- @[simp, grind =]
+  -- theorem hcomp_ren_left
+  --   [RenMap S] [RenMap T] [SubstMap S T]
+  --   (r : Ren) (σ : Subst T)
+  --   : (@Ren.to S r) ◾ σ = r.to
+  -- := by
+  --   funext; case _ x =>
+  --   induction x <;> simp [Subst.hcompose, Ren.to]
+
+  @[simp, grind =]
+  theorem hrewrite2 [SubstMap S T] {σ : Subst T} : (id S) ◾ σ = +0 := by simp [hcompose, id]
+
+  @[simp, grind =]
+  theorem hrewrite3 [SubstMap S T] {σ : Subst T} : (succ S) ◾ σ = +1 := by simp [hcompose, succ]
+
+  @[simp, grind =]
+  theorem hrewrite4
+    [SubstMap S T]
+    {x} {σ : Subst S} {τ : Subst T}
+    : (re x :: σ) ◾ τ = re x :: (σ ◾ τ)
+  := by
+    simp [Subst.hcompose]; congr
+    funext; case _ i =>
+    cases i <;> simp [Subst.cons]
+
+  @[grind =]
+  theorem hcomp_dist_ren_left
+    [SubstMap S T]
+    (r : Ren S) {σ : Subst S} {τ : Subst T}
+    : (r ∘ σ) ◾ τ = r ∘ σ ◾ τ
+  := by
+    funext; case _ x =>
+    simp [hcompose, compose_ren_left]
+
+  @[simp, grind =]
+  theorem hrewrite5
+    [SubstMap S T] [SubstMap T T] [SubstMapCompose S T]
+    {σ : Subst S} {τ μ : Subst T}
+    : (σ ◾ τ) ◾ μ = σ ◾ (τ ∘ μ)
+  := by
+    simp [Subst.hcompose]
+    funext; case _ x =>
+    generalize zdef : σ.act x = z
+    cases z <;> simp
+
+  @[grind =]
+  theorem hcomp_distr_ren_right
+    [RenMap S S] [SubstMap S S] [SubstMap S T] [SubstMapRenCommute S T]
+    (r : Ren S) (σ : Subst S) (μ : Subst T)
+    : (σ ∘ r) ◾ μ = (σ ◾ μ) ∘ r
+  := by
+    simp [hcompose, compose_ren_right]; funext; case _ x =>
+    generalize zdef : σ.act x = z
+    cases z <;> simp
+    rw [apply_ren_commute]
+
+  @[simp, grind =]
+  theorem apply_hcompose
+    [SubstMap S S] [SubstMap S T] [SubstMapHetCompose S T]
+    {s : S} {σ : Subst S} {τ : Subst T}
+    : s[σ][τ] = s[τ][σ ◾ τ]
+  := by exact SubstMapHetCompose.apply_hcompose
+
+  @[simp, grind =]
+  theorem hrewrite7
+    [SubstMap S S] [SubstMap S T] [SubstMapHetCompose S T]
+    {σ τ : Subst S} (μ : Subst T)
+    : (σ ∘ τ) ◾ μ = (σ ◾ μ) ∘ τ ◾ μ
+  := by
+    simp [Subst.hcompose, Subst.compose]
+    funext; case _ x =>
+    generalize zdef : σ.act x = z
+    cases z <;> simp [Subst.hcompose]
+
+  theorem hrewrite_lift1
+    [RenMap S S] [SubstMap S S] [SubstMap S T] [SubstMapHetCompose S T] [SubstMapRenCommute S T]
+    {σ : Subst S} {τ : Subst T}
+    : (σ ◾ τ).lift = σ.lift ◾ τ
+  := by
+    simp [Subst.lift]; congr; funext; case _ i =>
+    cases i <;> simp
+    case _ n =>
+      generalize zdef : σ.act n = z
+      cases z <;> simp; case _ t =>
+      rw [SubstMapRenCommute.apply_ren_commute]
+
+  @[simp, grind =]
+  theorem hrewrite_lift
+    [RenMap S S] [SubstMap S S] [SubstMap S T] [RenMapId S S] [RenMapCompose S S]
+    [SubstMapHetCompose S T] [SubstMapRenCommute S T]
+    {k} {σ : Subst S} {τ : Subst T}
+    : (σ ◾ τ).lift k = σ.lift k ◾ τ
+  := by
+    induction k generalizing σ τ
+    case _ => simp
+    case _ i ih =>
+      rw [rewrite_lift_succ]
+      rw [rewrite_lift_succ]
+      simp; rw [ih, hrewrite_lift1]
+      grind
+end Subst
+
+@[grind =]
+theorem Subst.compose_commute_succ [RenMap T T] {τ : Subst T}
+  : τ ∘ Ren.succ T = Ren.succ T ∘ τ.lift
+:= by congr
+
+@[grind =]
+theorem Ren.compose_commute_succ {r : Ren T} : r ∘ succ T = succ T ∘ r.lift := by simp [compose]
+
+theorem Subst.rewrite_lift_compose_ren_left_k1 [RenMap T T] {r : Ren T} {τ : Subst T}
+  : (r ∘ τ).lift = r.lift ∘ τ.lift
+:= by
+  simp [compose_ren_left, lift, Ren.lift]
+  funext; case _ x =>
+  cases x <;> simp
+
+@[simp, grind =]
+theorem Subst.rewrite_lift_compose_ren_left
+  [RenMap T T] [RenMapId T T] [RenMapCompose T T]
+  {k} {r : Ren T} {τ : Subst T}
+  : (r ∘ τ).lift k = r.lift k ∘ τ.lift k
+:= by
+  induction k generalizing r τ; congr
+  case _ k ih =>
+    rw [rewrite_lift_succ, ih]
+    rw [rewrite_lift_compose_ren_left_k1]
+    rw [<-rewrite_lift_succ]
+    rw [<-Ren.lift_of_succ]
+
+theorem Subst.lift_compose_ren_right_k1
+  [RenMap T T] [RenMapId T T] [RenMapCompose T T]
+  {σ : Subst T} {r : Ren T}
+  : (σ ∘ r).lift = σ.lift ∘ r.lift
+:= by
+  simp [lift]; congr; funext; case _ x =>
+  cases x <;> simp; case _ x =>
+  grind
+
+@[simp, grind =]
+theorem Subst.lift_compose_ren_right
+  [RenMap T T] [RenMapId T T] [RenMapCompose T T]
+  {k} {σ : Subst T} {r : Ren T}
+  : (σ ∘ r).lift k = σ.lift k ∘ r.lift k
+:= by
+  induction k generalizing σ r; simp
+  case _ k ih =>
+    rw [rewrite_lift_succ, ih]
+    rw [lift_compose_ren_right_k1]
+    rw [<-rewrite_lift_succ]
+    rw [<-Ren.lift_of_succ]
+
+theorem Subst.rewrite_lift_compose_k1
+  [RenMap T T] [SubstMap T T] [SubstMapRenComposeLeft T T] [SubstMapRenComposeRight T]
+  {σ τ : Subst T}
+  : (σ ∘ τ).lift = σ.lift ∘ τ.lift
+:= by
+  simp [compose, lift]
+  funext; case _ x =>
+  cases x <;> simp
+  case _ x =>
+  cases σ.act x <;> simp; case _ t =>
+  rw [SubstMapRenComposeLeft.apply_ren_compose_left]
+  rw [SubstMapRenComposeRight.apply_ren_compose_right]
+  have lem := Subst.compose_commute_succ (τ := τ)
+  simp [lift] at lem
+  rw [lem]
+
+@[simp, grind =]
+theorem Subst.rewrite_lift_compose
+  [RenMap T T] [RenMapId T T] [RenMapCompose T T] [SubstMap T T]
+  [SubstMapRenComposeLeft T T] [SubstMapRenComposeRight T]
+  {k} {σ τ : Subst T}
+  : (σ ∘ τ).lift k = σ.lift k ∘ τ.lift k
+:= by
+  induction k generalizing σ τ; simp
+  case _ k ih =>
+    rw [rewrite_lift_succ, ih]
+    rw [rewrite_lift_succ (σ := σ)]
+    rw [rewrite_lift_succ (σ := τ)]
+    rw [rewrite_lift_compose_k1]
+
+macro "subst_solve_id" : tactic => `(tactic| {
+  intro t; induction t
+  any_goals solve | simp +instances [*]
+  all_goals try simp at *; simp  +instances [*]; grind
+})
+
+macro "subst_solve_stable" : tactic => `(tactic| {
+  intro r σ h
+  funext; case _ t =>
+  induction t generalizing r σ
+  all_goals simp [rmap, smap, *] at *; try simp +instances [*]
+  any_goals solve | (rw [<-h]; simp +instances [Ren.to])
+  all_goals try repeat funext; grind
+})
+
+macro "subst_solve_compose" : tactic => `(tactic| {
+  intro s σ τ
+  induction s generalizing σ τ
+  any_goals solve | simp +instances [*]
+  try any_goals solve | (
+    try simp [-Subst.rewrite_lift, *]
+    try funext; case _ x =>
+    try rw [<-Ren.to_lift]
+    try simp [-Subst.rewrite_lift, *]
+    try grind)
+})
+
+end LeanSubst
