LeanSubst/Types/Option.lean
@@ -1,0 +1,51 @@
+
+import LeanSubst.Laws
+
+namespace LeanSubst
+
+universe u1 u2 u3
+variable {S : Type u1} {T : Type u2} {U : Type u3}
+
+def Option.rmap [i : RenMap S T] (r : Ren T) : Option S -> Option S
+| none => none
+| some t => some t⟨r⟩
+
+instance [RenMap S T] : RenMap (Option S) T where
+  rmap := Option.rmap
+
+@[simp, grind =]
+theorem Option.rmap_none [RenMap S T] {r : Ren T} : (@Option.none S)⟨r⟩ = none := by
+  simp [RenMap.rmap, Option.rmap]
+
+@[simp, grind =]
+theorem Option.rmap_some [RenMap S T] {x : S} {r : Ren T} : (some x)⟨r⟩ = some x⟨r⟩ := by
+  simp [RenMap.rmap, Option.rmap]
+
+instance [RenMap S T] [RenMapId S T] : RenMapId (Option S) T where
+  apply_id := by intro t; cases t <;> simp
+
+instance [RenMap S T] [RenMapCompose S T] : RenMapCompose (Option S) T where
+  apply_compose := by intro s σ τ; cases s <;> simp
+
+def Option.smap [SubstMap S T] (σ : Subst T) : Option S -> Option S
+| none => none
+| some t => some t[σ]
+
+instance [SubstMap S T] : SubstMap (Option S) T where
+  smap := Option.smap
+
+@[simp, grind =]
+theorem Option.smap_none [SubstMap S T] {σ : Subst T} : (@Option.none S)[σ] = none := by
+  simp [SubstMap.smap, Option.smap]
+
+@[simp, grind =]
+theorem Option.smap_some [SubstMap S T] {x : S} {σ : Subst T} : (some x)[σ] = some x[σ] := by
+  simp [SubstMap.smap, Option.smap]
+
+instance [RenMap S T] [SubstMap S T] [SubstMapId S T] : SubstMapId (Option S) T where
+  apply_id := by intro t; cases t <;> simp
+
+instance [SubstMap T T] [SubstMap S T] [SubstMapCompose S T] : SubstMapCompose (Option S) T where
+  apply_compose := by intro s σ τ; cases s <;> simp
+
+end LeanSubst
